coq_translation/default/examples/generics/generics_associated_types_problem.v
@@ -80,12 +80,10 @@ Module
         (A := i32)
         (B := i32)
       := {
-    generics_associated_types_problem.Contains.contains
-      `{H' : State.Trait}
+    generics_associated_types_problem.Contains.contains `{H' : State.Trait}
       :=
       contains;
-    generics_associated_types_problem.Contains.first
-      `{H' : State.Trait}
+    generics_associated_types_problem.Contains.first `{H' : State.Trait}
       :=
       first;
     generics_associated_types_problem.Contains.last `{H' : State.Trait} := last;
